# 736.lisp-语法解析

```ts
/*
 * @lc app=leetcode.cn id=736 lang=typescript
 *
 * [736] Lisp 语法解析
 */

// @lc code=start
function evaluate(s: string): number {}
// @lc code=end
```

## 解法 1: 模拟

```ts
function evaluate(s: string): number {
  const n = s.length
  type ArgType = { [key: string]: number }

  const dfs = (start: number, args: ArgType = {}): [number, number] => {
    const val: ArgType = {}
    let op = '',
      ch = '',
      vals: number[] = [],
      res = -1
    for (let i = start, j = start; i < n; i = ++j) {
      if (s[i] === ' ') continue
      let cur = s[i]
      if (cur === '(') {
        const [next, v] = dfs(i + 1, { ...args, ...val })
        j = next
        if (op === 'let') {
          if (ch === '') res = v
          else {
            val[ch] = v
            ch = ''
          }
        } else {
          vals.push(v)
        }
      } else if (cur === ')') {
        if (op === 'let') {
          if (res === -1) {
            if (/[a-z]/.test(ch[0])) {
              return [j, val[ch]]
            } else {
              return [j, Number(ch)]
            }
          } else {
            return [j, res]
          }
        } else if (op === 'add') {
          return [j, vals[0] + vals[1]]
        } else {
          return [j, vals[0] * vals[1]]
        }
      } else {
        while (j + 1 < n && s[j + 1] !== ' ' && s[j + 1] !== ')') cur += s[++j]

        if (op === '') op = cur
        else {
          if (op === 'let') {
            if (ch === '') ch = cur
            else {
              if (/[a-z]/.test(cur[0])) {
                val[ch] = val[cur]
              } else {
                val[ch] = Number(cur)
              }
              ch = ''
            }
          } else if (op === 'add' || op === 'mult') {
            if (/[a-z]/.test(cur[0])) {
              vals.push(args[cur])
            } else {
              vals.push(Number(cur))
            }
          }
        }
      }
    }
    return [-1, -1]
  }

  return dfs(1)[1]
}
```

## Case

```ts
test.each([
  { input: { expression: '(let x -2 y x y)' }, output: -2 },
  { input: { expression: '(let x 7 -12)' }, output: -12 },
  { input: { expression: '(let a1 3 b2 (add a1 1) b2)' }, output: 4 },
  { input: { expression: '(let x 2 (mult x (let x 3 y 4 (add x y))))' }, output: 14 },
  { input: { expression: '(let x 3 x 2 x)' }, output: 2 },
  { input: { expression: '(let x 1 y 2 x (add x y) (add x y))' }, output: 5 },
])('input: expression = $input.expression', ({ input: { expression }, output }) => {
  expect(evaluate(expression)).toEqual(output)
})
```
